low/MonadTactics.v
@@ -5,13 +5,24 @@ Set Implicit Arguments.
 Require Export Monads Loops.
 
 
-(** * Updating the type of a result **)
+(** * Some useful definitions **)
+
+(** Aborting results **)
 
 Definition aborting_result A (r : result A) :=
   match r with
   | result_success _ _ => false
   | _ => true
   end.
+
+Definition impossible_result A (r : result A) :=
+  match r with
+  | result_impossible_stack _ _ _ => true
+  | _ => false
+  end.
+
+
+(** ** Updating the type of a result **)
 
 Definition convert_type_monad A B (r : result A) :
     aborting_result r ->
@@ -42,7 +53,8 @@ Lemma convert_type_monad_transitive : forall A B C (r : result A) H1 H2,
   = (convert_type_monad r H1 : result C).
 Proof. introv. destruct r; (reflexivity || inverts~ H1). Qed.
 
-(** This tactic tries to simplify as much as can be threaded versions of [convert_type_monad]. **)
+(** This tactic tries to simplify as much as can be threaded versions
+  of [convert_type_monad]. **)
 Ltac clean_convert_type_one :=
   let term_trans A C r H1 := constr:(@convert_type_monad A C r H1) in
   match goal with
@@ -57,6 +69,115 @@ Ltac clean_convert_type_one :=
   end.
 
 Ltac clean_convert_type := repeat clean_convert_type_one.
+
+
+(** ** Getting the parameters of an impossible result **)
+
+Definition get_impossible_stack_state A (r : result A) :=
+  match r with
+  | result_impossible_stack S0 _ _ => S0
+  | _ => arbitrary
+  end.
+
+Definition get_impossible_stack_stack A (r : result A) :=
+  match r with
+  | result_impossible_stack _ st _ => st
+  | _ => arbitrary
+  end.
+
+Definition get_impossible_stack_message A (r : result A) :=
+  match r with
+  | result_impossible_stack _ _ msg => msg
+  | _ => arbitrary
+  end.
+
+Lemma rewrite_impossible_result : forall A (r : result A),
+  impossible_result r ->
+  r = result_impossible_stack
+        (get_impossible_stack_state r)
+        (get_impossible_stack_stack r)
+        (get_impossible_stack_message r).
+Proof. introv I. destruct r; tryfalse. reflexivity. Qed.
+
+
+(** ** Some useful tactics **)
+
+Ltac destruct_PrimSxp_struct p :=
+  let p_offset := fresh p "offset" in
+  destruct p as [p_offset].
+
+Ltac destruct_SymSxp_struct s :=
+  let s_pname := fresh s "pname" in
+  let s_value := fresh s "value" in
+  let s_internal := fresh s "internal" in
+  destruct s as [s_pname s_value s_internal].
+
+Ltac destruct_ListSxp_struct l :=
+  let l_carval := fresh l "carval" in
+  let l_cdrval := fresh l "cdrval" in
+  let l_tagval := fresh l "tagval" in
+  destruct l as [l_carval l_cdrval l_tagval].
+
+Ltac destruct_EnvSxp_struct e :=
+  let e_frame := fresh e "frame" in
+  let e_enclos := fresh e "enclos" in
+  destruct e as [e_frame e_enclos].
+
+Ltac destruct_CloSxp_struct c :=
+  let c_formals := fresh c "formals" in
+  let c_body := fresh c "body" in
+  let c_env := fresh c "env" in
+  destruct c as [c_formals c_body c_env].
+
+Ltac destruct_PromSxp_struct p :=
+  let p_value := fresh p "value" in
+  let p_expr := fresh p "expr" in
+  let p_env := fresh p "env" in
+  destruct p as [p_value p_expr p_env].
+
+Ltac destruct_NonVector_SExpRec_aux deep e_ :=
+  let e_header := fresh e_ "header" in
+  let e_data := fresh e_ "data" in
+  destruct e_ as [e_header e_data];
+  let e_prim := fresh e_ "prim" in
+  let e_sym := fresh e_ "sym" in
+  let e_list := fresh e_ "list" in
+  let e_env := fresh e_ "env" in
+  let e_clo := fresh e_ "clo" in
+  let e_prom := fresh e_ "prom" in
+  let inner t e_i :=
+    match deep with
+    | true => t e_i
+    | false => idtac
+    end in
+  destruct e_data as [ e_prim | e_sym | e_list | e_env | e_clo | e_prom ];
+    [ inner destruct_PrimSxp_struct e_prim
+    | inner destruct_SymSxp_struct e_sym
+    | inner destruct_ListSxp_struct e_list
+    | inner destruct_EnvSxp_struct e_env
+    | inner destruct_CloSxp_struct e_clo
+    | inner destruct_PromSxp_struct e_prom ].
+
+Ltac destruct_NonVector_SExpRec_deep := destruct_NonVector_SExpRec_aux true.
+Ltac destruct_NonVector_SExpRec := destruct_NonVector_SExpRec_aux false.
+
+Ltac destruct_SExpRec_aux deep1 deep2 e_ :=
+  let e_nonVector := fresh e_ "nonVector" in
+  let e_vectorChar := fresh e_ "vectorChar" in
+  let e_vectorInteger := fresh e_ "vectorInteger" in
+  let e_vectorComplex := fresh e_ "vectorComplex" in
+  let e_vectorReal := fresh e_ "vectorReal" in
+  let e_vectorPointer := fresh e_ "vectorPointer" in
+  destruct e_ as [ e_nonVector | e_vectorChar | e_vectorInteger
+                 | e_vectorComplex | e_vectorReal | e_vectorPointer];
+  [ match deep1 with
+    | true => destruct_NonVector_SExpRec_aux deep2 e_nonVector
+    | false => idtac
+    end | .. ].
+
+Ltac destruct_SExpRec_deep := destruct_SExpRec_aux true false.
+Ltac destruct_SExpRec_deep_full := destruct_SExpRec_aux true true.
+Ltac destruct_SExpRec := destruct_SExpRec_aux false false.
 
 
 (** * Simplifying monads **)
@@ -96,11 +217,137 @@ Lemma if_defined_aborts : forall A B S (cont : state -> A -> result B),
 Proof. reflexivity. Qed.
 
 Definition if_defined_abort : forall A B S (cont : state -> A -> result B),
-    let%defined a := None using S in cont S a
-    = result_impossible_stack S _ _
-  := fun _ _ _ _ => eq_refl.
+    impossible_result (let%defined a := None using S in cont S a).
+Proof. reflexivity. Qed.
 
-(* TODO: From [if_is_prim], maybe tactics for read and write. *)
+Lemma if_is_prim_pass : forall A S header offset (cont : _ -> _ -> result A),
+  let%prim a_, a_prim :=
+    make_NonVector_SExpRec header (make_PrimSxp_struct offset) using S in
+    cont a_ a_prim
+  = cont (make_NonVector_SExpRec header (make_PrimSxp_struct offset))
+      (make_PrimSxp_struct offset).
+Proof. reflexivity. Qed.
+
+Lemma if_is_prim_aborts : forall A S (e_ : SExpRec) (cont : _ -> _ -> result A),
+  (forall header offset,
+    e_ <> make_NonVector_SExpRec header (make_PrimSxp_struct offset)) ->
+  aborting_result (let%prim a_, a_prim := e_ using S in cont a_ a_prim).
+Proof. introv D. destruct_SExpRec_deep_full e_; (reflexivity || false~ D). Qed.
+
+Lemma if_is_prim_abort : forall A S (e_ : SExpRec) (cont : _ -> _ -> result A),
+  (forall header offset,
+    e_ <> make_NonVector_SExpRec header (make_PrimSxp_struct offset)) ->
+  impossible_result (let%prim a_, a_prim := e_ using S in cont a_ a_prim).
+Proof. introv D. destruct_SExpRec_deep_full e_; (reflexivity || false~ D). Qed.
+
+Lemma if_is_sym_pass : forall A S header pname value internal (cont : _ -> _ -> result A),
+  let%sym a_, a_sym :=
+    make_NonVector_SExpRec header (make_SymSxp_struct pname value internal) using S in
+    cont a_ a_sym
+  = cont (make_NonVector_SExpRec header (make_SymSxp_struct pname value internal))
+      (make_SymSxp_struct pname value internal).
+Proof. reflexivity. Qed.
+
+Lemma if_is_sym_aborts : forall A S (e_ : SExpRec) (cont : _ -> _ -> result A),
+  (forall header pname value internal,
+    e_ <> make_NonVector_SExpRec header (make_SymSxp_struct pname value internal)) ->
+  aborting_result (let%sym a_, a_sym := e_ using S in cont a_ a_sym).
+Proof. introv D. destruct_SExpRec_deep_full e_; (reflexivity || false~ D). Qed.
+
+Lemma if_is_sym_abort : forall A S (e_ : SExpRec) (cont : _ -> _ -> result A),
+  (forall header pname value internal,
+    e_ <> make_NonVector_SExpRec header (make_SymSxp_struct pname value internal)) ->
+  impossible_result (let%sym a_, a_sym := e_ using S in cont a_ a_sym).
+Proof. introv D. destruct_SExpRec_deep_full e_; (reflexivity || false~ D). Qed.
+
+Lemma if_is_list_pass : forall A S header car cdr tag (cont : _ -> _ -> result A),
+  let%list a_, a_list :=
+    make_NonVector_SExpRec header (make_ListSxp_struct car cdr tag) using S in
+    cont a_ a_list
+  = cont (make_NonVector_SExpRec header (make_ListSxp_struct car cdr tag))
+      (make_ListSxp_struct car cdr tag).
+Proof. reflexivity. Qed.
+
+Lemma if_is_list_aborts : forall A S (e_ : SExpRec) (cont : _ -> _ -> result A),
+  (forall header car cdr tag,
+    e_ <> make_NonVector_SExpRec header (make_ListSxp_struct car cdr tag)) ->
+  aborting_result (let%list a_, a_list := e_ using S in cont a_ a_list).
+Proof. introv D. destruct_SExpRec_deep_full e_; (reflexivity || false~ D). Qed.
+
+Lemma if_is_list_abort : forall A S (e_ : SExpRec) (cont : _ -> _ -> result A),
+  (forall header car cdr tag,
+    e_ <> make_NonVector_SExpRec header (make_ListSxp_struct car cdr tag)) ->
+  impossible_result (let%list a_, a_list := e_ using S in cont a_ a_list).
+Proof. introv D. destruct_SExpRec_deep_full e_; (reflexivity || false~ D). Qed.
+
+Lemma if_is_env_pass : forall A S header frame enclos (cont : _ -> _ -> result A),
+  let%env a_, a_env :=
+    make_NonVector_SExpRec header (make_EnvSxp_struct frame enclos) using S in
+    cont a_ a_env
+  = cont (make_NonVector_SExpRec header (make_EnvSxp_struct frame enclos))
+      (make_EnvSxp_struct frame enclos).
+Proof. reflexivity. Qed.
+
+Lemma if_is_env_aborts : forall A S (e_ : SExpRec) (cont : _ -> _ -> result A),
+  (forall header frame enclos,
+    e_ <> make_NonVector_SExpRec header (make_EnvSxp_struct frame enclos)) ->
+  aborting_result (let%env a_, a_env := e_ using S in cont a_ a_env).
+Proof. introv D. destruct_SExpRec_deep_full e_; (reflexivity || false~ D). Qed.
+
+Lemma if_is_env_abort : forall A S (e_ : SExpRec) (cont : _ -> _ -> result A),
+  (forall header frame enclos,
+    e_ <> make_NonVector_SExpRec header (make_EnvSxp_struct frame enclos)) ->
+  impossible_result (let%env a_, a_env := e_ using S in cont a_ a_env).
+Proof. introv D. destruct_SExpRec_deep_full e_; (reflexivity || false~ D). Qed.
+
+Lemma if_is_clo_pass : forall A S header formals body env (cont : _ -> _ -> result A),
+  let%clo a_, a_clo :=
+    make_NonVector_SExpRec header (make_CloSxp_struct formals body env) using S in
+    cont a_ a_clo
+  = cont (make_NonVector_SExpRec header (make_CloSxp_struct formals body env))
+      (make_CloSxp_struct formals body env).
+Proof. reflexivity. Qed.
+
+Lemma if_is_clo_aborts : forall A S (e_ : SExpRec) (cont : _ -> _ -> result A),
+  (forall header formals body env,
+    e_ <> make_NonVector_SExpRec header (make_CloSxp_struct formals body env)) ->
+  aborting_result (let%clo a_, a_clo := e_ using S in cont a_ a_clo).
+Proof. introv D. destruct_SExpRec_deep_full e_; (reflexivity || false~ D). Qed.
+
+Lemma if_is_clo_abort : forall A S (e_ : SExpRec) (cont : _ -> _ -> result A),
+  (forall header formals body env,
+    e_ <> make_NonVector_SExpRec header (make_CloSxp_struct formals body env)) ->
+  impossible_result (let%clo a_, a_clo := e_ using S in cont a_ a_clo).
+Proof. introv D. destruct_SExpRec_deep_full e_; (reflexivity || false~ D). Qed.
+
+Lemma if_is_prom_pass : forall A S header value expr env (cont : _ -> _ -> result A),
+  let%prom a_, a_prom :=
+    make_NonVector_SExpRec header (make_PromSxp_struct value expr env) using S in
+    cont a_ a_prom
+  = cont (make_NonVector_SExpRec header (make_PromSxp_struct value expr env))
+      (make_PromSxp_struct value expr env).
+Proof. reflexivity. Qed.
+
+Lemma if_is_prom_aborts : forall A S (e_ : SExpRec) (cont : _ -> _ -> result A),
+  (forall header value expr env,
+    e_ <> make_NonVector_SExpRec header (make_PromSxp_struct value expr env)) ->
+  aborting_result (let%prom a_, a_prom := e_ using S in cont a_ a_prom).
+Proof. introv D. destruct_SExpRec_deep_full e_; (reflexivity || false~ D). Qed.
+
+Lemma if_is_prom_abort : forall A S (e_ : SExpRec) (cont : _ -> _ -> result A),
+  (forall header value expr env,
+    e_ <> make_NonVector_SExpRec header (make_PromSxp_struct value expr env)) ->
+  impossible_result (let%prom a_, a_prom := e_ using S in cont a_ a_prom).
+Proof. introv D. destruct_SExpRec_deep_full e_; (reflexivity || false~ D). Qed.
+
+(* TODO: From [read_as_prim]. Although these probably won’t get any
+  useful lemmae without the paths of Path.v because of reading operations. *)
+
+(* TODO: [let_Vector*], [read_nth_cell_Vector*] *)
+
+(* TODO: map%* using the paths. *)
+
+(* TODO: All the monads of Loops.v. *)
 
 
 (** ** Tactics **)
@@ -110,6 +357,12 @@ Ltac get_pass_lemma t :=
   | add_stack => constr:(add_stack_pass)
   | if_success => constr:(if_success_pass)
   | if_defined => constr:(if_defined_pass)
+  | if_is_prim => constr:(if_is_prim_pass)
+  | if_is_sym => constr:(if_is_sym_pass)
+  | if_is_list => constr:(if_is_list_pass)
+  | if_is_env => constr:(if_is_env_pass)
+  | if_is_clo => constr:(if_is_clo_pass)
+  | if_is_prom => constr:(if_is_prom_pass)
   end.
 
 Ltac get_aborts_lemma t :=
@@ -117,15 +370,33 @@ Ltac get_aborts_lemma t :=
   | add_stack => constr:(add_stack_aborts)
   | if_success => constr:(if_success_aborts)
   | if_defined => constr:(if_defined_aborts)
+  | if_is_prim => constr:(if_is_prim_aborts)
+  | if_is_sym => constr:(if_is_sym_aborts)
+  | if_is_list => constr:(if_is_list_aborts)
+  | if_is_env => constr:(if_is_env_aborts)
+  | if_is_clo => constr:(if_is_clo_aborts)
+  | if_is_prom => constr:(if_is_prom_aborts)
   end.
 
 Ltac get_abort_lemma t :=
   match get_head t with
   | if_success => constr:(if_success_abort)
   | if_defined => constr:(if_defined_abort)
+  | if_is_prim => constr:(if_is_prim_abort)
+  | if_is_sym => constr:(if_is_sym_abort)
+  | if_is_list => constr:(if_is_list_abort)
+  | if_is_env => constr:(if_is_env_abort)
+  | if_is_clo => constr:(if_is_clo_abort)
+  | if_is_prom => constr:(if_is_prom_abort)
   end.
 
-(** To speed up computations, we directly fail if a result is not already fully computed. **)
+Ltac unfolds_get_impossible :=
+  try unfolds get_impossible_stack_state;
+  try unfolds get_impossible_stack_stack;
+  try unfolds get_impossible_stack_message.
+
+(** To speed up computations, we directly fail if a result is not
+  already fully computed. **)
 Ltac result_computed r :=
   match get_head r with
   | result_success => idtac
@@ -136,37 +407,52 @@ Ltac result_computed r :=
   | result_bottom => idtac
   end.
 
-Ltac munfold_with_result t r :=
+Ltac try_solving_premises :=
+  try solve [
+    intros;
+    first [
+        reflexivity
+      | discriminate
+      | autos~ ] ].
+
+Ltac munfold_with_subresult t r :=
   result_computed r;
   first [
       let P := get_pass_lemma t in
-      rewrite~ P
+      rewrite P; try_solving_premises
     | let A := get_abort_lemma t in
       first [
-          rewrite A
+          rewrite A; try_solving_premises
+        | rewrite rewrite_impossible_result with (r := t);
+          [| apply A; try_solving_premises ];
+          unfolds_get_impossible
         | let H := fresh "Habort" in
           asserts H: (aborting_result r);
           [ first [
                 reflexivity
               | let AT := get_aborts_lemma t in
-                apply* AT ]
+                apply AT; try_solving_premises ]
           | rewrite A with H ] ] ].
 
-Ltac munfold_without_result t :=
+Ltac munfold_without_subresult t :=
   first [
       let P := get_pass_lemma t in
-      rewrite~ P
+      rewrite P; try_solving_premises
     | let A := get_abort_lemma t in
-      rewrite A ].
+      first [
+          rewrite A; try_solving_premises
+        | rewrite rewrite_impossible_result with (r := t);
+          [| apply A; try_solving_premises ];
+          unfolds_get_impossible ] ].
 
 Ltac munfold :=
   match goal with
   | |- context [ add_stack ?fname ?r ] =>
-    munfold_with_result (add_stack fname r) r
+    munfold_with_subresult (add_stack fname r) r
   | |- context [ if_success ?r ?cont ] =>
-    munfold_with_result (if_success r cont) r
+    munfold_with_subresult (if_success r cont) r
   | |- context [ if_defined ?S ?o ?cont ] =>
-    munfold_without_result (if_defined S o cont)
+    munfold_without_subresult (if_defined S o cont)
   | |- context [ result_skip ?S ] =>
     unfolds result_skip
   | |- context [ if_then_else_success ?b ?c1 ?c2 ] =>
@@ -175,7 +461,10 @@ Ltac munfold :=
     unfolds if_then_success
   | |- context [ if_option_defined ?c ?cont1 ?cont2 ] =>
     unfolds if_option_defined
+  | |- context [ if_is_prim ?S ?e_ ?cont ] =>
+    munfold_without_subresult (if_is_prim S e_ cont)
   end.
 
 Ltac munfolds :=
   repeat (munfold; repeat let_simpl).
+
